changed the notation to denote elementwise

src/Decomposition.v
@@ -4,63 +4,6 @@ Require Import Syntax Semantics.
 
 Set Implicit Arguments.
 
-Definition DomainSubset A B (s1: M.t A) (s2: M.t B) := forall k, M.In k s1 -> M.In k s2.
-
-Section MapSet.
-  Variable A: Type.
-  Variable p: M.key -> A -> option A.
-
-  Definition rmModify k v m := match p k v with
-                                 | None => m
-                                 | Some v' => M.add k v' m
-                               end.
-  Definition liftToMap1 s :=
-    M.fold rmModify s (M.empty _).
-
-  Theorem liftToMap1Empty: liftToMap1 (M.empty _) = M.empty _.
-  Proof.
-    unfold liftToMap1, M.fold; reflexivity.
-  Qed.
-
-  Lemma liftToMap1Subset s: DomainSubset (liftToMap1 s) s.
-  Proof.
-    apply (M.map_induction (P := fun s => DomainSubset (liftToMap1 s) s)); unfold DomainSubset; intros.
-    - rewrite liftToMap1Empty in *.
-      intuition.
-    - unfold liftToMap1 in H1.
-      rewrite M.F.P.fold_add in H1; fold (liftToMap1 m) in *; unfold rmModify. (* intuition. *)
-      + apply M.F.P.F.add_in_iff.
-        unfold rmModify in *.
-        destruct (p k v).
-        apply M.F.P.F.add_in_iff in H1.
-        destruct H1; intuition.
-        right; apply (H _ H1).
-      + intuition.
-      + clear; unfold Morphisms.Proper, Morphisms.respectful; intros; subst.
-        apply M.leibniz in H1; subst.
-        intuition.
-      + clear; unfold M.F.P.transpose_neqkey; intros.
-        unfold rmModify.
-        destruct (p k e), (p k' e');
-          try apply M.transpose_neqkey_Equal_add; intuition.
-      + intuition.
-  Qed.
-        
-  Theorem liftToMap1AddOne k v:
-    liftToMap1 (M.add k v (M.empty _)) =
-    match p k v with
-      | Some argRet => M.add k argRet (M.empty _)
-      | None => M.empty _
-    end.
-  Proof.
-    case_eq (p k v); unfold liftToMap1, rmModify, M.fold; simpl.
-    intros a H.
-    rewrite H; reflexivity.
-    intros H.
-    rewrite H; reflexivity.
-  Qed.
-End MapSet.
-
 Section Decomposition.
   Variable imp spec: Modules.
   Variable theta: RegsT -> RegsT.
